src/HOL/Theorie.v
@@ -6,142 +6,6 @@ Import ListNotations.
 
 (*Reserved Notation "Γ | Ξ ⊢⟨ n ⟩ φ" (at level 88).*)
 
-Definition shift11 {n : nat} (g : fin (S n)) : fin (S (S n)).
-Proof.
-  destruct g.
-  - apply Some. apply Some. apply f.
-  - apply None.
-Defined.
-
-Lemma typ_shift : forall (n : nat) (Γ : HOL_ctx n)
-                         (s s' s0: st) (t : tm (S n)),
-    s .: Γ ⊢⟨ S n ⟩ t ~: s0 ->
-    s .: (s' .: Γ) ⊢⟨ S (S n) ⟩ ren_tm shift11 t ~: s0.
-Proof.
-  intros. apply (typ_ren (S (S n)) (S n) shift11 (s .: (s' .: Γ)) (s .: Γ)).
-  intro. unfold ">>"; simpl. case f; reflexivity.
-  apply H.
-Qed.
-
-Definition ex_tm {n : nat} (s : st) (φ : tm (S n)) : tm n.
-Proof.
-  apply forall_tm. apply ℙₛ. apply imp_tm.
-  apply forall_tm. apply s. apply imp_tm.
-  exact (ren_tm shift11 φ). apply var_tm. apply Some. apply None.
-  apply var_tm. apply None.
-Defined.
-
-Notation "∃ₛ" := (ex_tm) (at level 80).
-
-Lemma typ_ex_tm : forall (n : nat) (Γ : HOL_ctx n) (s : st) (φ : tm (S n)),
-    s .: Γ ⊢⟨ S n ⟩ φ ~: ℙₛ -> Γ ⊢⟨ n ⟩ ∃ₛ s φ ~: ℙₛ.
-Proof.
-  intros. apply typ_forall.
-  constructor. apply typ_forall. constructor.
-  apply typ_shift. apply H.
-  constructor. constructor.
-Qed.
-
-Definition eq_tm {n : nat} (s : st) (t : tm n) (u : tm n) : tm n.
-Proof.
-  apply forall_tm. apply (s →ₛ ℙₛ). apply imp_tm.
-  apply app_tm. apply var_tm; apply None.
-  exact (ren_tm shift t).
-  apply app_tm. apply var_tm; apply None.
-  exact (ren_tm shift u).
-Defined.
-
-Notation "t =⟨ s ⟩ u" := (eq_tm s t u) (at level 77).
-
-Lemma typ_eq_tm : forall (n : nat) (Γ : HOL_ctx n) (s : st)
-                         (t : tm n) (u : tm n),
-    Γ ⊢⟨ n ⟩ t ~: s -> Γ ⊢⟨ n ⟩ u ~: s -> Γ ⊢⟨ n ⟩ t =⟨ s ⟩ u ~: ℙₛ.
-Proof.
-  intros. apply typ_forall.
-  constructor. apply (typ_app s).
-  constructor. apply typ_weaken. apply H.
-  apply (typ_app s). constructor. apply typ_weaken. apply H0.
-Qed.
-
-Definition or_tm {n : nat} (t u : tm n) : tm n.
-Proof.
-  apply forall_tm. apply ℙₛ. apply imp_tm.
-  apply imp_tm.
-  exact (ren_tm shift t). apply var_tm. apply None.
-  apply imp_tm. apply imp_tm.
-  exact (ren_tm shift u). apply var_tm. apply None.
-  apply var_tm. apply None.
-Defined.
-
-Notation "φ ∨ₛ ψ" := (or_tm φ ψ) (at level 80).
-
-Lemma typ_eq_or : forall (n : nat) (Γ : HOL_ctx n) (t u : tm n),
-    Γ ⊢⟨ n ⟩ t ~: ℙₛ -> Γ ⊢⟨ n ⟩ u ~: ℙₛ -> Γ ⊢⟨ n ⟩ t ∨ₛ u ~: ℙₛ.
-Proof.
-  intros. apply typ_forall. constructor.
-  constructor. apply typ_weaken. apply H.
-  constructor. constructor. constructor. apply typ_weaken.
-  apply H0. constructor. constructor.
-Qed.
-
-Definition and_tm {n : nat} (t u : tm n) : tm n.
-Proof.
-  apply forall_tm. apply ℙₛ. apply imp_tm. apply imp_tm.
-  apply (ren_tm shift t).
-  apply imp_tm. apply (ren_tm shift u). apply var_tm. apply None.
-  apply var_tm. apply None.
-Defined.
-
-Notation "φ ∧ₛ ψ" := (and_tm φ ψ) (at level 79).
-
-Lemma typ_and : forall (n : nat) (Γ : HOL_ctx n) (φ ψ : tm n),
-    Γ ⊢⟨ n ⟩ φ ~: ℙₛ -> Γ ⊢⟨ n ⟩ ψ ~: ℙₛ -> Γ ⊢⟨ n ⟩ φ ∧ₛ ψ ~: ℙₛ.
-Proof.
-  intros. constructor.
-  constructor. constructor. apply typ_weaken. apply H.
-  constructor. apply typ_weaken. apply H0.
-  constructor. constructor.
-Qed.
-
-Definition true_tm {n : nat} : tm n.
-Proof.
-  apply forall_tm. apply ℙₛ. apply imp_tm. apply var_tm. apply None.
-  apply var_tm. apply None.
-Defined.
-
-Notation "⊤ₛ" := (true_tm).
-
-Lemma typ_true : forall (n : nat) (Γ : HOL_ctx n),
-    Γ ⊢⟨ n ⟩ ⊤ₛ ~: ℙₛ.
-Proof.
-  intros. apply (typ_forall ℙₛ). repeat constructor.
-Qed.
-
-Definition false_tm {n : nat} : tm n.
-Proof.
-  apply forall_tm. apply ℙₛ. apply var_tm. apply None.
-Defined.
-
-Notation "⊥ₛ" := (false_tm).
-
-Lemma typ_false : forall (n : nat) (Γ : HOL_ctx n),
-    Γ ⊢⟨ n ⟩ ⊥ₛ ~: ℙₛ.
-Proof.
-  intros. apply (typ_forall ℙₛ). constructor.
-Qed.
-
-Definition not_tm {n : nat} (t : tm n) : tm n.
-Proof.
-  apply imp_tm. apply t. apply ⊥ₛ.
-Defined.
-
-Notation "¬ₛ φ" := (not_tm φ) (at level 79).
-
-Lemma typ_not : forall (n : nat) (Γ : HOL_ctx n) (φ : tm n),
-    Γ ⊢⟨ n ⟩ φ ~: ℙₛ -> Γ ⊢⟨ n ⟩ ¬ₛ φ ~: ℙₛ.
-Proof.
-  intros. constructor. apply H. apply typ_false.
-Qed.
 
 Require Import CRM.Prelude.ListCRM.
 
@@ -152,40 +16,52 @@ Definition wt_ctx {n : nat} {Γ : HOL_ctx n} (Ξ : proof_ctx n Γ) : Prop :=
 
 Inductive proving : forall (n : nat) (Γ : HOL_ctx n)
                            (Ξ : proof_ctx n Γ) (φ : tm n), Prop :=
-| ax : forall {n : nat} {Γ : HOL_ctx n}
-              {Ξ : proof_ctx n Γ} {φ : tm n},
+| pr_ax : forall {n : nat} {Γ : HOL_ctx n}
+                 {Ξ : proof_ctx n Γ} {φ : tm n},
     wt_ctx Ξ -> In φ Ξ -> proving n Γ Ξ φ
-| transp : forall {n : nat} {Γ : HOL_ctx n}
-                  {Ξ : proof_ctx n Γ} {φ ψ : tm n},
+| pr_transp : forall {n : nat} {Γ : HOL_ctx n}
+                     {Ξ : proof_ctx n Γ} (φ : tm n)
+                     {ψ : tm n},
     proving n Γ Ξ φ -> Γ ⊢⟨ n ⟩ ψ ~: ℙₛ ->
     φ =ₛ ψ -> proving n Γ Ξ ψ
-| abs : forall {n : nat} {Γ : HOL_ctx n}
-               {Ξ : proof_ctx n Γ} {φ ψ : tm n},
+| pr_abs : forall {n : nat} {Γ : HOL_ctx n}
+                  {Ξ : proof_ctx n Γ} {φ ψ : tm n},
     proving n Γ (φ :: Ξ) ψ -> proving n Γ Ξ (φ ⇒ₛ ψ)
-| app : forall {n : nat} {Γ : HOL_ctx n}
-               {Ξ : proof_ctx n Γ} {φ ψ : tm n},
+| pr_app : forall {n : nat} {Γ : HOL_ctx n}
+                  {Ξ : proof_ctx n Γ} (φ : tm n)
+                  {ψ : tm n},
     proving n Γ Ξ (φ ⇒ₛ ψ) -> proving n Γ Ξ φ ->
     proving n Γ Ξ ψ
-| abs_f : forall {n : nat} {Γ : HOL_ctx n} {Ξ : proof_ctx n Γ}
-                 {φ : tm (S n)} {s : st},
+| pr_abs_f : forall {n : nat} {Γ : HOL_ctx n} {Ξ : proof_ctx n Γ}
+                    {φ : tm (S n)} {s : st},
     proving (S n) (s .: Γ) (List.map (ren_tm shift) Ξ) φ ->
     proving n Γ Ξ (∀ₛ s φ)
-| app_f : forall {n : nat} {Γ : HOL_ctx n} {Ξ : proof_ctx n Γ}
-                 {φ : tm (S n)} {t : tm n} {s : st},
+| pr_app_f : forall {n : nat} {Γ : HOL_ctx n} {Ξ : proof_ctx n Γ}
+                    {φ : tm (S n)} (t : tm n) (s : st),
     proving n Γ Ξ (∀ₛ s φ) -> Γ ⊢⟨ n ⟩ t ~: s ->
-    proving n Γ Ξ (φ [t .: (fun v => ⟦ v ⟧ₛ)]).
-
-Lemma proving_refl :
-  forall (n : nat) (Γ : HOL_ctx n) (Ξ : proof_ctx n Γ)
-         (t : tm n) (s : st),
-    wt_ctx Ξ -> Γ ⊢⟨ n ⟩ t ~: s -> proving n Γ Ξ (t =⟨ s ⟩ t).
-Proof.
-  intros. unfold eq_tm. apply abs_f.
-  apply abs. apply ax. constructor.
-  apply (typ_app s). constructor. apply typ_weaken; apply H0.
-  apply (map_forall _ _ (ren_tm shift) (fun x => typ_weaken n Γ x ℙₛ (s →ₛ ℙₛ))).
-  apply H. simpl. left; reflexivity.
-Qed.
+    proving n Γ Ξ (φ [t .: (fun v => ⟦ v ⟧ₛ)])
+| pr_recN : forall {n : nat} {Γ : HOL_ctx n} {Ξ : proof_ctx n Γ}
+                   {φ : tm n},
+    proving n Γ Ξ (φ @ₛ Zₛ) ->
+    proving n Γ Ξ
+      (∀ₛ ℕₛ ((ren_tm shift φ @ₛ ((S n) __tm var_zero)) ⇒ₛ
+                (ren_tm shift φ @ₛ (Sₛ ((S n) __tm var_zero))))) ->
+    proving n Γ Ξ (∀ₛ ℕₛ (ren_tm shift φ @ₛ ((S n) __tm var_zero)))
+| pr_recB : forall {n : nat} {Γ : HOL_ctx n} {Ξ : proof_ctx n Γ}
+                   {φ : tm n},
+    proving n Γ Ξ (φ @ₛ ttₛ) ->
+    proving n Γ Ξ (φ @ₛ ffₛ) ->
+    proving n Γ Ξ (∀ₛ 𝔹ₛ (ren_tm shift φ @ₛ ((S n) __tm var_zero)))
+| pr_recL : forall {n : nat} {Γ : HOL_ctx n} {Ξ : proof_ctx n Γ}
+                   {s : st} {φ : tm n},
+    proving n Γ Ξ (φ @ₛ []ₛ) ->
+    proving n Γ Ξ
+      (∀ₛ s
+        (∀ₛ (𝕃ₛ s)
+          (ren_tm (shift >> shift) φ @ₛ
+             (((S (S n)) __tm (shift var_zero)) ::ₛ
+             ((S (S n)) __tm var_zero))))) ->
+    proving n Γ Ξ (∀ₛ (𝕃ₛ s) (ren_tm shift φ @ₛ ((S n) __tm var_zero))).
 
 Lemma wt_proving :
   forall (n : nat) (Γ : HOL_ctx n) (Ξ : proof_ctx n Γ) (φ : tm n),
@@ -214,6 +90,33 @@ Proof.
     asimpl. intro f; case f eqn:e.
     asimpl. apply typ_var. asimpl. apply H0.
     dependent destruction H2. apply H2.
+  - destruct IHproving1 as [H1 H2]. split; [apply H1|].
+    constructor. apply (typ_app ℕₛ).
+    apply typ_weaken. dependent destruction H2.
+    dependent destruction H2_0. apply H2_.
+    constructor.
+  - destruct IHproving1 as [H1 H2]. split; [apply H1|].
+    constructor. apply (typ_app 𝔹ₛ).
+    apply typ_weaken. dependent destruction H2.
+    dependent destruction H2_0. apply H2_.
+    constructor.
+  - destruct IHproving1 as [H1 H2]. split; [apply H1|].
+    constructor. apply (typ_app (𝕃ₛ s)).
+    apply typ_weaken. dependent destruction H2.
+    dependent destruction H2_0.
+    destruct IHproving2 as [_ H3].
+    dependent destruction H3. dependent destruction H3.
+    dependent destruction H3.
+    dependent destruction H3_0.
+    dependent destruction H3_0_1.
+    simpl in H3_.
+    assert (ren_tm (shift >> shift) φ =
+              ren_tm shift (ren_tm shift φ)).
+    asimpl; reflexivity.
+    apply (typ_weaken_rev _ _ _ _ s).
+    apply (typ_weaken_rev _ _ _ _ (𝕃ₛ s)).
+    asimpl. apply H3_.
+    constructor.
 Qed.
 
 Lemma ren_proof :
@@ -223,16 +126,19 @@ Lemma ren_proof :
     proving n Γ Ξ φ -> proving m Δ (map (ren_tm ξ) Ξ) (ren_tm ξ φ).
 Proof.
   intros; revert m Δ ξ H; induction H0; intros; simpl.
-  - apply ax.
+  - apply pr_ax.
     apply (map_forall _ _ (ren_tm ξ)
              (fun x => typ_ren m n ξ Δ Γ x _ H1)).
     apply H. apply (in_map (ren_tm ξ) Ξ φ H0).
-  -
-  - simpl; apply abs. apply IHproving. apply H.
+  - apply (ren_βeq n m φ ψ ξ) in H1.
+    apply (pr_transp (ren_tm ξ φ)).
+    apply IHproving. apply H2. apply (typ_ren _ _ ξ Δ Γ).
+    apply H2. apply H. apply H1.
+  - simpl; apply pr_abs. apply IHproving. apply H.
   - simpl. specialize (IHproving1 _ _ _ H).
     specialize (IHproving2 _ _ _ H).
-    apply (app IHproving1 IHproving2).
-  - asimpl. apply abs_f.
+    apply (pr_app _ IHproving1 IHproving2).
+  - asimpl. apply pr_abs_f.
     specialize (IHproving _ (s .: Δ) (var_zero .: ξ >> shift)).
     asimpl in IHproving.
     rewrite map_map in IHproving. asimpl in IHproving.
@@ -250,8 +156,30 @@ Proof.
     asimpl in IHproving.
     assert (Δ ⊢⟨ m ⟩ ren_tm ξ t ~: s).
     apply (typ_ren _ _ _ _ _ _ _ H1 H).
-    specialize (app_f IHproving H2); intro.
+    specialize (pr_app_f _ _ IHproving H2); intro.
     asimpl in H3. apply H3.
+  - asimpl.
+    specialize (IHproving1 m Δ ξ H); specialize (IHproving2 m Δ ξ H).
+    asimpl in IHproving2.
+    specialize (@pr_recN m Δ (map (ren_tm ξ) Ξ) (ren_tm ξ φ) IHproving1).
+    intro H0. asimpl in H0. apply H0.
+    apply IHproving2.
+  - asimpl.
+    specialize (IHproving1 m Δ ξ H).
+    specialize (IHproving2 m Δ ξ H).
+    asimpl in IHproving1; asimpl in IHproving2.
+    specialize (pr_recB IHproving1 IHproving2).
+    asimpl. trivial.
+  - asimpl.
+    specialize (IHproving1 m Δ ξ H).
+    specialize (IHproving2 m Δ ξ H).
+    asimpl in IHproving1; simpl in IHproving2.
+    specialize (@pr_recL m Δ (map (ren_tm ξ) Ξ) s (ren_tm ξ φ)).
+    asimpl. intro H0; specialize (H0 IHproving1).
+    apply H0.
+    unfold ">>" in IHproving2.
+    asimpl in IHproving2.
+    apply IHproving2.
 Qed.
 
 Lemma subst_proof :
@@ -261,18 +189,23 @@ Lemma subst_proof :
     proving m Γ (map (subst_tm v) Ξ) (φ [ v ]).
 Proof.
   intros n m v Γ Δ Ξ φ Hv Hφ; revert m v Γ Hv; induction Hφ; intros; simpl.
-  - apply ax.
+  - apply pr_ax.
     apply (map_forall (fun x => Γ  ⊢⟨ n ⟩ x ~: ℙₛ)
              (fun x => Γ0 ⊢⟨ m ⟩ x ~: ℙₛ)).
     intro a. apply comp_typ_vec.
     apply Hv. apply H.
     apply (in_map (subst_tm v) Ξ φ H0).
-  - asimpl. apply abs. apply IHHφ.
+  - apply (subst_βeq n m φ ψ v) in H0.
+    apply (pr_transp (subst_tm v φ)).
+    apply IHHφ. apply Hv.
+    apply (comp_typ_vec _ _ v Γ0 Γ).
+    apply Hv. apply H. apply H0.
+  - asimpl. apply pr_abs. apply IHHφ.
     apply Hv.
   - specialize (IHHφ1 _ _ _ Hv).
     specialize (IHHφ2 _ _ _ Hv).
-    apply (app IHHφ1 IHHφ2).
-  - asimpl. apply abs_f.
+    apply (pr_app _ IHHφ1 IHHφ2).
+  - asimpl. apply pr_abs_f.
     specialize (IHHφ (S m) ((S m)__tm var_zero .: v >> ren_tm shift)
                   (s .: Γ0)).
     asimpl in IHHφ.
@@ -288,7 +221,7 @@ Proof.
     rewrite <- H0. apply IHHφ.
   - asimpl. specialize (IHHφ m v Γ0 Hv).
     asimpl in IHHφ.
-    apply (@app_f _ _ _ _ (t [v])) in IHHφ.
+    apply (@pr_app_f _ _ _ _ (t [v])) in IHHφ.
     asimpl in IHHφ.
     assert (φ [t[v] .: v >> (ren_tm shift >> subst_tm (t[v] .: m __tm))] = φ[t[v] .: v]).
     apply ext_tm.
@@ -296,4 +229,84 @@ Proof.
     asimpl. reflexivity. reflexivity.
     apply (eq_rec _ (proving m Γ0 (map (subst_tm v) Ξ)) IHHφ _ H0).
     apply (comp_typ_vec _ _ _ _ _ _ _ Hv H).
+  - specialize (IHHφ1 m v Γ0 Hv). specialize (IHHφ2 m v Γ0 Hv).
+    asimpl. asimpl in IHHφ1. asimpl in IHHφ2.
+    assert (subst_tm (v >> ren_tm shift) φ = ren_tm shift (subst_tm v φ)).
+    asimpl. reflexivity.
+    rewrite H in IHHφ2.
+    specialize (pr_recN IHHφ1 IHHφ2).
+    asimpl. trivial.
+  - asimpl; asimpl in IHHφ1; asimpl in IHHφ2.
+    specialize (pr_recB (IHHφ1 _ _ _ Hv) (IHHφ2 _ _ _ Hv)).
+    asimpl. trivial.
+  - specialize (IHHφ1 m v Γ0 Hv); specialize (IHHφ2 m v Γ0 Hv).
+    asimpl; asimpl in IHHφ1; asimpl in IHHφ2.
+    assert
+      (subst_tm
+         (shift >>
+            (((S m)__tm var_zero .: v >> ren_tm shift) >>
+               ren_tm shift)) φ =
+         ren_tm (shift >> shift) (subst_tm v φ)).
+    asimpl. apply ext_tm.
+    intro; unfold ">>"; asimpl.
+    reflexivity.
+    rewrite H in IHHφ2; clear H.
+    specialize (pr_recL IHHφ1 IHHφ2).
+    asimpl. trivial.
+Qed.
+
+Lemma weaken_proof :
+  forall (n : nat) (Γ : HOL_ctx n)
+         (Ξ Θ : proof_ctx n Γ) (φ : tm n),
+    proving n Γ Ξ φ -> incl Ξ Θ ->
+    wt_ctx Θ -> proving n Γ Θ φ.
+Proof.
+  intros; revert Θ H0 H1; induction H; intros.
+  - apply pr_ax. apply H2. apply H1.
+    apply H0.
+  - apply (pr_transp φ). apply IHproving.
+    apply H2. apply H3. apply H0. apply H1.
+  - apply pr_abs. apply IHproving.
+    intro χ. intro χφΞ.
+    simpl; simpl in χφΞ.
+    destruct χφΞ as [ φχ | χΞ ].
+    left; apply φχ.
+    right; apply (H0 _ χΞ).
+    constructor.
+    destruct (wt_proving n Γ (φ :: Ξ) ψ H) as [H2 _].
+    inversion H2. apply H5.
+    apply H1.
+  - apply (pr_app φ). apply IHproving1.
+    apply H1. apply H2. apply IHproving2.
+    apply H1. apply H2.
+  - apply pr_abs_f. apply IHproving.
+    intro x.
+    intro xΞ. rewrite in_map_iff. rewrite in_map_iff in xΞ.
+    destruct xΞ. exists x0. destruct H2.
+    split; [apply H2|].
+    apply H0. apply H3.
+    apply (map_forall _ _ (ren_tm shift)
+             (fun x => typ_weaken n Γ x _ _) Θ H1).
+  - apply (pr_app_f t s).
+    apply IHproving. apply H1. apply H2.
+    apply H0.
+  - apply pr_recN. apply IHproving1. apply H1. apply H2.
+    apply IHproving2. apply H1. apply H2.
+  - apply pr_recB. apply IHproving1. apply H1. apply H2.
+    apply IHproving2. apply H1. apply H2.
+  - apply pr_recL. apply IHproving1. apply H1. apply H2.
+    apply IHproving2. apply H1. apply H2.
+Qed.
+
+Lemma weaken_proof_1 :
+  forall (n : nat) (Γ : HOL_ctx n)
+         (Ξ : proof_ctx n Γ) (φ ψ : tm n),
+    proving n Γ Ξ φ -> Γ ⊢⟨ n ⟩ ψ ~: ℙₛ ->
+    proving n Γ (ψ :: Ξ) φ.
+Proof.
+  intros.
+  apply (weaken_proof n Γ Ξ (ψ :: Ξ)).
+  apply H. intros x xΞ; simpl; right; apply xΞ.
+  constructor. apply H0.
+  apply (wt_proving n Γ Ξ φ H).
 Qed.
