src/HOL/Logical.v
@@ -1,0 +1,220 @@
+From CRM Require Import Base Typing Reduction Theorie fintype.
+Import CombineNotations SubstNotations.
+From CRM Require Import Prelude.ListCRM.
+
+Require Import PeanoNat List.
+
+Definition shift11 {n : nat} (g : fin (S n)) : fin (S (S n)).
+Proof.
+  destruct g.
+  - apply Some. apply Some. apply f.
+  - apply None.
+Defined.
+
+Lemma typ_shift : forall (n : nat) (Γ : HOL_ctx n)
+                         (s s' s0: st) (t : tm (S n)),
+    s .: Γ ⊢⟨ S n ⟩ t ~: s0 ->
+    s .: (s' .: Γ) ⊢⟨ S (S n) ⟩ ren_tm shift11 t ~: s0.
+Proof.
+  intros. apply (typ_ren (S (S n)) (S n) shift11 (s .: (s' .: Γ)) (s .: Γ)).
+  intro. unfold ">>"; simpl. case f; reflexivity.
+  apply H.
+Qed.
+
+Definition ex_tm {n : nat} (s : st) (φ : tm (S n)) : tm n.
+Proof.
+  apply forall_tm. apply ℙₛ. apply imp_tm.
+  apply forall_tm. apply s. apply imp_tm.
+  exact (ren_tm shift11 φ). apply var_tm. apply Some. apply None.
+  apply var_tm. apply None.
+Defined.
+
+Notation "∃ₛ" := (ex_tm) (at level 80).
+
+Lemma typ_ex : forall {n : nat} {Γ : HOL_ctx n} {φ : tm (S n)} (s : st),
+    s .: Γ ⊢⟨ S n ⟩ φ ~: ℙₛ -> Γ ⊢⟨ n ⟩ ∃ₛ s φ ~: ℙₛ.
+Proof.
+  intros. apply typ_forall.
+  constructor. apply typ_forall. constructor.
+  apply typ_shift. apply H.
+  constructor. constructor.
+Qed.
+
+Definition eq_tm {n : nat} (s : st) (t : tm n) (u : tm n) : tm n.
+Proof.
+  apply forall_tm. apply (s →ₛ ℙₛ). apply imp_tm.
+  apply app_tm. apply var_tm; apply None.
+  exact (ren_tm shift t).
+  apply app_tm. apply var_tm; apply None.
+  exact (ren_tm shift u).
+Defined.
+
+Notation "t =⟨ s ⟩ u" := (eq_tm s t u) (at level 77).
+
+Lemma typ_eq : forall {n : nat} {Γ : HOL_ctx n} (s : st)
+                         {t u : tm n},
+    Γ ⊢⟨ n ⟩ t ~: s -> Γ ⊢⟨ n ⟩ u ~: s -> Γ ⊢⟨ n ⟩ t =⟨ s ⟩ u ~: ℙₛ.
+Proof.
+  intros. apply typ_forall.
+  constructor. apply (typ_app s).
+  constructor. apply typ_weaken. apply H.
+  apply (typ_app s). constructor. apply typ_weaken. apply H0.
+Qed.
+
+Definition or_tm {n : nat} (φ ψ : tm n) : tm n.
+Proof.
+  apply forall_tm. apply ℙₛ. apply imp_tm.
+  apply imp_tm.
+  exact (ren_tm shift φ). apply var_tm. apply None.
+  apply imp_tm. apply imp_tm.
+  exact (ren_tm shift ψ). apply var_tm. apply None.
+  apply var_tm. apply None.
+Defined.
+
+Notation "φ ∨ₛ ψ" := (or_tm φ ψ) (at level 80).
+
+Lemma typ_or : forall {n : nat} {Γ : HOL_ctx n} {φ ψ : tm n},
+    Γ ⊢⟨ n ⟩ φ ~: ℙₛ -> Γ ⊢⟨ n ⟩ ψ ~: ℙₛ -> Γ ⊢⟨ n ⟩ φ ∨ₛ ψ ~: ℙₛ.
+Proof.
+  intros. apply typ_forall. constructor.
+  constructor. apply typ_weaken. apply H.
+  constructor. constructor. constructor. apply typ_weaken.
+  apply H0. constructor. constructor.
+Qed.
+
+Definition and_tm {n : nat} (φ ψ : tm n) : tm n.
+Proof.
+  apply forall_tm. apply ℙₛ. apply imp_tm. apply imp_tm.
+  apply (ren_tm shift φ).
+  apply imp_tm. apply (ren_tm shift ψ). apply var_tm. apply None.
+  apply var_tm. apply None.
+Defined.
+
+Notation "φ ∧ₛ ψ" := (and_tm φ ψ) (at level 79).
+
+Lemma typ_and : forall {n : nat} {Γ : HOL_ctx n} {φ ψ : tm n},
+    Γ ⊢⟨ n ⟩ φ ~: ℙₛ -> Γ ⊢⟨ n ⟩ ψ ~: ℙₛ -> Γ ⊢⟨ n ⟩ φ ∧ₛ ψ ~: ℙₛ.
+Proof.
+  intros. constructor.
+  constructor. constructor. apply typ_weaken. apply H.
+  constructor. apply typ_weaken. apply H0.
+  constructor. constructor.
+Qed.
+
+Definition true_tm {n : nat} : tm n.
+Proof.
+  apply forall_tm. apply ℙₛ. apply imp_tm. apply var_tm. apply None.
+  apply var_tm. apply None.
+Defined.
+
+Notation "⊤ₛ" := (true_tm).
+
+Lemma typ_true : forall {n : nat} (Γ : HOL_ctx n),
+    Γ ⊢⟨ n ⟩ ⊤ₛ ~: ℙₛ.
+Proof.
+  intros. apply (typ_forall ℙₛ). repeat constructor.
+Qed.
+
+Definition false_tm {n : nat} : tm n.
+Proof.
+  apply forall_tm. apply ℙₛ. apply var_tm. apply None.
+Defined.
+
+Notation "⊥ₛ" := (false_tm).
+
+Lemma typ_false : forall {n : nat} (Γ : HOL_ctx n),
+    Γ ⊢⟨ n ⟩ ⊥ₛ ~: ℙₛ.
+Proof.
+  intros. apply (typ_forall ℙₛ). constructor.
+Qed.
+
+Definition not_tm {n : nat} (φ : tm n) : tm n.
+Proof.
+  apply imp_tm. apply φ. apply ⊥ₛ.
+Defined.
+
+Notation "¬ₛ φ" := (not_tm φ) (at level 79).
+
+Lemma typ_not : forall {n : nat} {Γ : HOL_ctx n} {φ : tm n},
+    Γ ⊢⟨ n ⟩ φ ~: ℙₛ -> Γ ⊢⟨ n ⟩ ¬ₛ φ ~: ℙₛ.
+Proof.
+  intros. constructor. apply H. apply typ_false.
+Qed.
+
+Definition relat_forall_tm {n : nat} (s : st) (φ : tm (S n))
+  : tm n.
+Proof.
+  apply forall_tm. apply s. apply imp_tm.
+  apply sort_tm. apply s. apply var_tm. apply var_zero.
+  apply φ.
+Defined.
+
+Notation "∀{ s } φ" := (relat_forall_tm s φ) (at level 80).
+
+Lemma typ_relat_forall :
+  forall {n : nat} {Γ : HOL_ctx n} (s : st) {φ : tm (S n)},
+    s .: Γ ⊢⟨ S n ⟩ φ ~: ℙₛ -> Γ ⊢⟨ n ⟩ ∀{ s } φ ~: ℙₛ.
+Proof.
+  intros. apply typ_forall. constructor.
+  constructor. constructor. apply H.
+Qed.
+
+Definition relat_ex_tm {n : nat} (s : st) (φ : tm (S n)) : tm n.
+Proof.
+  apply ex_tm. apply s. apply and_tm.
+  apply sort_tm. apply s. apply var_tm. apply var_zero.
+  apply φ.
+Defined.
+
+Notation "∃{ s } φ" := (relat_ex_tm s φ) (at level 80).
+
+Lemma typ_relat_ex :
+  forall {n : nat} {Γ : HOL_ctx n} (s : st) {φ : tm (S n)},
+    s .: Γ ⊢⟨ S n ⟩ φ ~: ℙₛ -> Γ ⊢⟨ n ⟩ ∃{ s } φ ~: ℙₛ.
+Proof.
+  intros. apply typ_ex. apply typ_and.
+  constructor. constructor. apply H.
+Qed.
+
+Lemma proving_refl :
+  forall {n : nat} {Γ : HOL_ctx n} {Ξ : proof_ctx n Γ}
+         {t : tm n} {s : st},
+    wt_ctx Ξ -> Γ ⊢⟨ n ⟩ t ~: s -> proving n Γ Ξ (t =⟨ s ⟩ t).
+Proof.
+  intros. unfold eq_tm. apply pr_abs_f.
+  apply pr_abs. apply pr_ax. constructor.
+  apply (typ_app s). constructor. apply typ_weaken; apply H0.
+  apply (map_forall _ _ (ren_tm shift) (fun x => typ_weaken n Γ x ℙₛ (s →ₛ ℙₛ))).
+  apply H. simpl. left; reflexivity.
+Qed.
+
+Lemma eq_elim :
+  forall {n : nat} {Γ : HOL_ctx n} {Ξ : proof_ctx n Γ}
+         {t : tm n} {u φ : tm n} {s : st},
+    proving n Γ Ξ (t =⟨ s ⟩ u) ->
+    Γ ⊢⟨ n ⟩ φ ~: s →ₛ ℙₛ ->
+    proving n Γ Ξ (φ @ₛ t) ->
+    proving n Γ Ξ (φ @ₛ u).
+Proof.
+  intros.
+  apply (pr_app_f φ (s →ₛ ℙₛ)) in H.
+  asimpl in H.
+  apply (pr_app (φ @ₛ t) H H1).
+  apply H0.
+Qed.
+
+Lemma def_eq_to_eq :
+  forall {n : nat} {Γ : HOL_ctx n} {Ξ : proof_ctx n Γ}
+         {t u : tm n} {s : st},
+    Γ ⊢⟨ n ⟩ t ~: s -> Γ ⊢⟨ n ⟩ u ~: s ->
+    t =ₛ u -> wt_ctx Ξ ->
+    proving n Γ Ξ (t =⟨ s ⟩ u).
+Proof.
+  intros. apply (pr_transp (t =⟨ s ⟩ t)).
+  apply proving_refl. apply H2.
+  apply H. apply typ_eq.
+  apply H. apply H0.
+  repeat apply βeq_compat.
+  apply ren_βeq.
+  apply H1.
+Qed.
