src/HOL/Termes.v
@@ -1,0 +1,195 @@
+From CRM Require Import Base Typing Reduction Theorie Logical fintype.
+Import CombineNotations SubstNotations.
+
+Require Import PeanoNat List.
+
+Fixpoint nat_to_tm {n : nat} (m : nat) : tm n :=
+  match m with
+  | 0 => Zₛ
+  | S p => Sₛ (nat_to_tm p)
+  end.
+
+Lemma typ_nat_to_tm :
+  forall {n : nat} (Γ : HOL_ctx n) (m : nat),
+    Γ ⊢⟨ n ⟩ nat_to_tm m ~: ℕₛ.
+Proof.
+  intros. induction m. constructor.
+  simpl. constructor. apply IHm.
+Qed.
+
+Definition restr_tm {n : nat} : tm n :=
+  ƛ (ƛ
+  (recℕₛ []ₛ
+    (ƛ (ƛ
+       ((⟦ (shift >> shift >> shift) var_zero ⟧ₛ @ₛ ⟦ shift var_zero ⟧ₛ)
+       ::ₛ ⟦ var_zero ⟧ₛ))) ⟦ var_zero ⟧ₛ)).
+
+Lemma typ_restr :
+  forall {n : nat} {Γ : HOL_ctx n} {s : st},
+    Γ ⊢⟨ n ⟩ restr_tm ~: (ℕₛ →ₛ s) →ₛ ℕₛ →ₛ 𝕃ₛ s.
+Proof.
+  intros. repeat constructor.
+  apply (typ_app ℕₛ).
+  repeat constructor. constructor.
+Qed.
+
+Definition length_tm {n : nat} : tm n :=
+  ƛ (rec𝕃ₛ Zₛ (ƛ (ƛ (ƛ (Sₛ ⟦ var_zero ⟧ₛ)))) ⟦ var_zero ⟧ₛ).
+
+Lemma typ_length :
+  forall {n : nat} {Γ : HOL_ctx n} (s : st),
+    Γ ⊢⟨ n ⟩ length_tm ~: (𝕃ₛ s) →ₛ ℕₛ.
+Proof.
+  intros. repeat constructor.
+  apply (typ_recL s); repeat constructor.
+Qed.
+
+Definition concat_tm {n : nat} : tm n :=
+  ƛ (rec𝕃ₛ (ƛ ⟦ var_zero ⟧ₛ)
+       (ƛ (ƛ (ƛ (ƛ (⟦ shift_p 3 var_zero ⟧ₛ ::ₛ (⟦ shift var_zero ⟧ₛ @ₛ ⟦ var_zero ⟧ₛ))))))
+       ⟦ var_zero ⟧ₛ).
+
+Lemma typ_concat :
+  forall {n : nat} {Γ : HOL_ctx n} {s : st},
+    Γ ⊢⟨ n ⟩ concat_tm ~: 𝕃ₛ s →ₛ 𝕃ₛ s →ₛ 𝕃ₛ s.
+Proof.
+  intros. repeat constructor.
+  apply (typ_recL s).
+  repeat constructor.
+  repeat constructor.
+  apply (typ_app (𝕃ₛ s)); repeat constructor.
+  constructor.
+Qed.
+
+Notation "t ++ₛ u" := (concat_tm @ₛ t @ₛ u) (at level 87).
+
+Definition pref_tm {n : nat} (s : st) : tm n :=
+  ƛ (ƛ (∃{𝕃ₛ s}
+         (⟦ shift var_zero ⟧ₛ =⟨ 𝕃ₛ s ⟩
+                                 (⟦ var_zero ⟧ₛ ++ₛ ⟦ shift_p 2 var_zero ⟧ₛ)))).
+
+Lemma typ_pref :
+  forall {n : nat} {Γ : HOL_ctx n} (s : st),
+    Γ ⊢⟨ n ⟩ pref_tm s ~: 𝕃ₛ s →ₛ 𝕃ₛ s →ₛ ℙₛ.
+Proof.
+  intros. constructor. constructor.
+  apply typ_relat_ex. apply typ_eq; repeat constructor.
+  apply (typ_app (𝕃ₛ s)). apply (typ_app (𝕃ₛ s)).
+  apply typ_concat.
+  constructor. constructor.
+Qed.
+
+Definition is_Tree_tm {n : nat} (s : st) : tm n :=
+  ƛ
+   (∀ₛ (𝕃ₛ s)
+     (∀ₛ (𝕃ₛ s)
+       ((pref_tm s @ₛ ⟦ shift var_zero ⟧ₛ @ₛ ⟦ var_zero ⟧ₛ) ⇒ₛ
+          ⟦ shift_p 2 var_zero ⟧ₛ @ₛ ⟦ var_zero ⟧ₛ ⇒ₛ
+          ⟦ shift_p 2 var_zero ⟧ₛ @ₛ ⟦ shift var_zero ⟧ₛ))).
+
+Lemma typ_is_Tree :
+  forall {n : nat} {Γ : HOL_ctx n} (s : st),
+    Γ ⊢⟨ n ⟩ is_Tree_tm s ~: ((𝕃ₛ s) →ₛ ℙₛ) →ₛ ℙₛ.
+Proof.
+  intros. repeat constructor.
+  apply (typ_app (𝕃ₛ s)).
+  apply (typ_app (𝕃ₛ s)).
+  apply typ_pref. constructor. constructor.
+  apply (typ_app (𝕃ₛ s)). constructor.
+  constructor.
+  apply (typ_app (𝕃ₛ s)). constructor.
+  constructor.
+Qed.
+
+Definition WKL_tm {n : nat} : tm n :=
+  ∀ₛ ((𝕃ₛ 𝔹ₛ) →ₛ ℙₛ)
+   (is_Tree_tm 𝔹ₛ @ₛ ⟦ var_zero ⟧ₛ ⇒ₛ
+      (∀{ ℕₛ }
+        (∃{ 𝕃ₛ 𝔹ₛ }
+          (((length_tm @ₛ ⟦ var_zero ⟧ₛ) =⟨ ℕₛ ⟩ ⟦ shift var_zero ⟧ₛ) ∧ₛ
+             (⟦ shift_p 2 var_zero ⟧ₛ @ₛ ⟦ var_zero⟧ₛ)))) ⇒ₛ
+      (∃{ ℕₛ →ₛ 𝔹ₛ }
+        (∀{ ℕₛ }
+          ((⟦ shift_p 2 var_zero ⟧ₛ @ₛ
+             (restr_tm @ₛ ⟦ shift var_zero ⟧ₛ @ₛ
+                ⟦ var_zero ⟧ₛ)))))).
+
+Lemma typ_WKL :
+  forall {n : nat} {Γ : HOL_ctx n},
+    Γ ⊢⟨ n ⟩ WKL_tm ~: ℙₛ.
+Proof.
+  intros. constructor. constructor.
+  apply (typ_app (𝕃ₛ 𝔹ₛ →ₛ ℙₛ)).
+  apply typ_is_Tree. constructor.
+  constructor.
+  apply typ_relat_forall. apply typ_relat_ex.
+  apply typ_and. apply (typ_eq ℕₛ).
+  apply (typ_app (𝕃ₛ 𝔹ₛ)). apply typ_length.
+  constructor. constructor.
+  apply (typ_app (𝕃ₛ 𝔹ₛ)); constructor.
+  apply typ_relat_ex. apply typ_relat_forall.
+  apply (typ_app (𝕃ₛ 𝔹ₛ)).
+  constructor.
+  apply (typ_app ℕₛ).
+  apply (typ_app (ℕₛ →ₛ 𝔹ₛ)).
+  apply typ_restr. constructor. constructor.
+Qed.
+
+Definition is_Mono_tm {n : nat} (s : st) : tm n :=
+  ƛ
+   (∀ₛ (𝕃ₛ s)
+     (∀ₛ (𝕃ₛ s)
+       ((pref_tm s @ₛ ⟦ shift var_zero ⟧ₛ @ₛ ⟦ var_zero ⟧ₛ) ⇒ₛ
+          ⟦ shift_p 2 var_zero ⟧ₛ @ₛ ⟦ shift var_zero ⟧ₛ ⇒ₛ
+          ⟦ shift_p 2 var_zero ⟧ₛ @ₛ ⟦ var_zero ⟧ₛ))).
+
+Lemma typ_is_Mono :
+  forall {n : nat} {Γ : HOL_ctx n} (s : st),
+    Γ ⊢⟨ n ⟩ is_Mono_tm s ~: ((𝕃ₛ s) →ₛ ℙₛ) →ₛ ℙₛ.
+Proof.
+  intros. repeat constructor.
+  apply (typ_app (𝕃ₛ s)).
+  apply (typ_app (𝕃ₛ s)).
+  apply typ_pref. constructor. constructor.
+  apply (typ_app (𝕃ₛ s)). constructor.
+  constructor.
+  apply (typ_app (𝕃ₛ s)). constructor.
+  constructor.
+Qed.
+
+Definition FT_tm {n : nat} : tm n :=
+  ∀ₛ ((𝕃ₛ 𝔹ₛ) →ₛ ℙₛ)
+   (is_Mono_tm 𝔹ₛ @ₛ ⟦ var_zero ⟧ₛ ⇒ₛ
+      (∀{ ℕₛ →ₛ 𝔹ₛ }
+        (∃{ ℕₛ }
+          (⟦ shift_p 2 var_zero ⟧ₛ @ₛ (restr_tm @ₛ ⟦ shift var_zero ⟧ₛ
+                                         @ₛ ⟦ var_zero ⟧ₛ)))) ⇒ₛ
+      (∃{ ℕₛ }
+        (∀{ ℕₛ →ₛ 𝔹ₛ }
+          (⟦ shift_p 2 var_zero ⟧ₛ @ₛ (restr_tm @ₛ ⟦ var_zero ⟧ₛ @ₛ
+                                         ⟦ shift var_zero ⟧ₛ))))).
+
+Lemma typ_FT :
+  forall {n : nat} {Γ : HOL_ctx n},
+    Γ ⊢⟨ n ⟩ FT_tm ~: ℙₛ.
+Proof.
+  intros. constructor. constructor.
+  apply (typ_app ((𝕃ₛ 𝔹ₛ) →ₛ ℙₛ)).
+  apply typ_is_Mono. constructor.
+  constructor.
+  apply typ_relat_forall. apply typ_relat_ex.
+  apply (typ_app (𝕃ₛ 𝔹ₛ)).
+  constructor.
+  apply (typ_app ℕₛ). apply (typ_app (ℕₛ →ₛ 𝔹ₛ)). apply typ_restr.
+  constructor. constructor.
+  apply typ_relat_ex. apply typ_relat_forall.
+  apply (typ_app (𝕃ₛ 𝔹ₛ)).
+  constructor.
+  apply (typ_app ℕₛ). apply (typ_app (ℕₛ →ₛ 𝔹ₛ)). apply typ_restr.
+  constructor. constructor.
+Qed.
+
+
+
+Theorem FT_nprove_WKL :
+  ~ (proving 0 (@False_rect st) (FT_tm :: nil) WKL_tm).
